src/OtDef.v
@@ -1,4 +1,5 @@
-Require Import Commons Basics ListTools.
+From Stdlib Require Import Basics.
+From OTRocq Require Import Commons ListTools.
 
 Section ExecAll.
 
